TlaDsl.lean
@@ -8,11 +8,13 @@ import TlaDsl.TlaVar
 import TlaDsl.Meta
 import TlaDsl.SimFull
 import TlaDsl.ModelCheck
+import TlaDsl.Pretty
 import TlaDsl.Examples.Counter
 import TlaDsl.Examples.Refinement
 import TlaDsl.Examples.TicketLock
 import TlaDsl.Examples.StrongFair
 import TlaDsl.Examples.Binders
+import TlaDsl.Examples.Processes
 import TlaDsl.Examples.Mutex
 import TlaDsl.Examples.ModelCheck
 import TlaDsl.Examples.Brackets
